cava/Cava/Signal.v
@@ -15,44 +15,147 @@
 (****************************************************************************)
 
 From Coq Require Import Strings.Ascii Strings.String.
+From Coq Require Import Lists.List.
+Import ListNotations.
 From Coq Require Import ZArith.ZArith.
 From Coq Require Import Vectors.Vector.
 
 From Cava Require Import Kind.
 From Cava Require Import VectorUtils.
 
-Inductive Signal : Kind -> Type :=
+(******************************************************************************)
+(* The types of signals that can flow over wires, used to index signal        *)
+(******************************************************************************)
+
+Inductive SignalType :=
+  | Void : SignalType                              (* An empty type *)
+  | Bit : SignalType                               (* A single wire *)
+  | Vec : SignalType -> nat -> SignalType          (* Vectors, possibly nested *)
+  | ExternalType : string -> SignalType.           (* An uninterpreted type *)
+
+(******************************************************************************)
+(* Combinational denotion of the SignalType and default values.               *)
+(******************************************************************************)
+
+Fixpoint combType (t: SignalType) : Type :=
+  match t with
+  | Void => unit
+  | Bit => bool
+  | Vec vt sz => Vector.t (combType vt) sz
+  | ExternalType _ => unit (* No semantics for combinational interpretation. *)
+  end.
+
+Fixpoint defaultCombValue (t: SignalType) : combType t :=
+  match t  with
+  | Void => tt
+  | Bit => false
+  | Vec t2 sz => Vector.const (defaultCombValue t2) sz
+  | ExternalType _ => tt
+  end.
+
+(******************************************************************************)
+(* Representation of circuit interface types with flat tuples.                *)
+(******************************************************************************)
+
+(* Right-associative tuples ending with a unit. *)
+
+Fixpoint tupleInterfaceR (signal: SignalType -> Type) (v : list SignalType) : Type :=
+  match v with
+  | [] => unit
+  | x :: pds => signal x * tupleInterfaceR signal pds
+  end.
+
+
+(* Left-associative tuples with no trailing unit. **)
+Fixpoint tupleInterface' (signal: SignalType -> Type) accum (l : list SignalType) : Type :=
+  match l with
+  | [] => accum
+  | x::xs => tupleInterface' signal (accum * signal x)%type xs
+  end.
+
+Definition tupleInterface (signal: SignalType -> Type) (l : list SignalType) : Type :=
+  match l with
+  | [] => unit
+  | x::xs => tupleInterface' signal (signal x) xs
+  end.
+
+(* Convert a right-associative tuple to a left-associative tuple. *)
+Fixpoint rebalance' (signal: SignalType -> Type)
+                    (ts : list SignalType) {accumT : Type} (accum : accumT)
+  : tupleInterfaceR signal ts -> tupleInterface' signal accumT ts :=
+  match ts with
+  | [] => fun _ : unit => accum
+  | x::xs =>
+    fun ab => rebalance' signal xs (accum, fst ab) (snd ab)
+  end.
+
+Definition rebalance (signal: SignalType -> Type)
+                      (ts : list SignalType)
+                      : tupleInterfaceR signal ts -> tupleInterface signal ts :=
+  match ts with
+  | [] => fun _ => tt
+  | x::xs => fun ab => rebalance' signal xs (fst ab) (snd ab)
+  end.
+
+(* Convert a left-associative tuple to a right-associative tuple. *)
+Fixpoint unbalance' (signal: SignalType -> Type)
+                    (ts : list SignalType) {accumT : Type}
+  : tupleInterface' signal accumT ts -> accumT * tupleInterfaceR signal ts :=
+  match ts with
+  | [] => fun (acc : accumT) => (acc, tt)
+  | x::xs =>
+    fun ab =>
+      let '(acc, vx, vxs) := unbalance' signal xs ab in
+      (acc, (vx, vxs))
+  end.
+
+Definition unbalance (signal: SignalType -> Type)
+                     (ts : list SignalType)
+                     : tupleInterface signal ts -> tupleInterfaceR signal ts :=
+  match ts as ts0 return tupleInterface signal ts0 -> tupleInterfaceR signal ts0 with
+  | [] => fun _ => tt
+  | x::xs => unbalance' signal xs
+  end.
+
+(******************************************************************************)
+(* Netlist AST representation for signal expressions.                         *)
+(******************************************************************************)
+
+Inductive Signal : SignalType -> Type :=
   | UndefinedSignal : Signal Void
   | UninterpretedSignal: forall {t: string}, string -> Signal (ExternalType t)
   | UninterpretedSignalIndex: forall (t: string), N -> Signal (ExternalType t)
-  | SelectField: forall {k1: Kind} (k2: Kind), Signal k1 -> string -> Signal k2
+  | SelectField: forall {t1: SignalType} (t2: SignalType), Signal t1 -> string -> Signal t2
   | Gnd: Signal Bit
   | Vcc: Signal Bit
   | Wire: N -> Signal Bit
   | NamedWire: string -> Signal Bit
-  | NamedVector: forall k s, string -> Signal (Vec k s)
-  | LocalVec: forall k s, N -> Signal (Vec k s)
-  | VecLit: forall {k s}, Vector.t (Signal k) s -> Signal (Vec k s)
+  | NamedVector: forall t s, string -> Signal (Vec t s)
+  | LocalVec: forall t s, N -> Signal (Vec t s)
+  | VecLit: forall {t s}, Vector.t (Signal t) s -> Signal (Vec t s)
   (* Dynamic index *)
-  | IndexAt:  forall {k sz isz}, Signal (Vec k sz) ->
-              Signal (Vec Bit isz) -> Signal k
+  | IndexAt:  forall {t sz isz}, Signal (Vec t sz) ->
+              Signal (Vec Bit isz) -> Signal t
   (* Static indexing *)
-  | IndexConst: forall {k sz}, Signal (Vec k sz) -> nat -> Signal k
+  | IndexConst: forall {t sz}, Signal (Vec t sz) -> nat -> Signal t
   (* Static slice *)
-  | Slice: forall {k sz} (start len: nat), Signal (Vec k sz) ->
-                                           Signal (Vec k len).
+  | Slice: forall {t sz} (start len: nat), Signal (Vec t sz) ->
+                                           Signal (Vec t len).
 
-(* A default unsmashed value for a given Kind. *)
-Fixpoint defaultKindSignal (k: Kind) : Signal k :=
-  match k with
+Definition denoteSignal (t : SignalType) : Type := Signal t.
+
+(* A default value for a given SignalType. *)
+Fixpoint defaultSignal (t: SignalType) : Signal t :=
+  match t with
   | Void => UndefinedSignal
   | Bit => Gnd
-  | Vec k s => VecLit (Vector.const (defaultKindSignal k) s)
-  | ExternalType s => UninterpretedSignal "default-error"
+  | Vec vt s => VecLit (Vector.const (defaultSignal vt) s)
+  | ExternalType s => UninterpretedSignal "default-defaultSignal"
   end.
 
-(* To allow us to represent a heterogenous list of Signal k values where
-   the Kind k varies we make a wrapper that erase the Kind index type.
+
+
+(* To allow us to represent a heterogenous list of Signal t values where
+   the Signal t varies we make a wrapper that erase the Kind index type.
 *)
 Inductive UntypedSignal := USignal : forall {Kind}, Signal Kind -> UntypedSignal.
-
