monad-examples/xilinx/XilinxAdderTree.v
@@ -31,16 +31,37 @@ Require Import Cava.Cava.
 Require Import Cava.Monad.CavaMonad.
 Require Import Cava.Monad.XilinxAdder.
 
-(******************************************************************************)
-(* A generic description of all adder trees made from a Xilinx adder          *)
-(* by using the tree combinator.                                              *)
-(******************************************************************************)
+Section WithCava.
+  Context {signal} `{Cava signal} `{Monad cava}.
 
-Definition adderTree {m bit} `{Cava m bit} {sz: nat}
-                     (default : bit)
-                     (n: nat) (v: Vector.t (Vector.t bit sz) (2^(S n))) :
-                     m (Vector.t bit sz) :=
-  tree (Vector.const default _) n xilinxAdder v.
+  (****************************************************************************)
+  (* A generic description of all adder trees made from a Xilinx adder        *)
+  (* by using the tree combinator.                                            *)
+  (****************************************************************************)
+  Definition adderTree {sz: nat}
+                       (n: nat) (v: signal (Vec (Vec Bit sz) (2^(S n)))):
+                      cava (signal (Vec Bit sz)) :=
+    z <- zero ;;
+    let def := unpeel (Vector.const z sz) in
+    tree def n xilinxAdder (peel v).
+
+  (****************************************************************************)
+  (* An adder tree with 2 inputs.                                             *)
+  (****************************************************************************)
+  Definition adderTree2 {sz: nat}
+                        (v : signal (Vec (Vec Bit sz) 2))
+                        : cava (signal (Vec Bit sz))
+    := adderTree 0 v.
+
+  (******************************************************************************)
+  (* An adder tree with 4 inputs.                                               *)
+  (******************************************************************************)
+  Definition adderTree4 {sz: nat}
+                        (v : signal (Vec (Vec Bit sz) 4))
+                        : cava (signal (Vec Bit sz))
+    := adderTree 1 v.
+
+End WithCava.
 
 (******************************************************************************)
 (* Some tests.                                                                *)
@@ -51,48 +72,27 @@ Definition v1 := N2Bv_sized 8 17.
 Definition v2 := N2Bv_sized 8  6.
 Definition v3 := N2Bv_sized 8  3.
 
-Local Open Scope N_scope.
-Local Open Scope string_scope.
-
-(******************************************************************************)
-(* An adder tree with 2 inputs.                                               *)
-(******************************************************************************)
-
 Local Open Scope nat_scope.
 Local Open Scope vector_scope.
 
-Definition adderTree2 {m bit} `{Cava m bit} {sz: nat}
-                      (default : bit)
-                      (v : Vector.t (Vector.t bit sz) 2) : m (Vector.t bit sz)
-  := adderTree default 0 v.
-
 Definition v0_v1 : Vector.t (Bvector 8) 2 := [v0; v1].
-Definition v0_plus_v1 : Bvector 8 := combinational (adderTree2 false v0_v1).
+Definition v0_plus_v1 : Bvector 8 := combinational (adderTree2 v0_v1).
 Example sum_vo_v1 : v0_plus_v1 = N2Bv_sized 8 21.
 Proof. reflexivity. Qed.
-
-(******************************************************************************)
-(* An adder tree with 4 inputs.                                               *)
-(******************************************************************************)
-
-Definition adderTree4 {m bit} `{Cava m bit} {sz: nat}
-                      (default : bit)
-                      (v : Vector.t (Vector.t bit sz) 4) : m (Vector.t bit sz)
-  := adderTree default 1 v.
 
 Local Open Scope N_scope.
 
 Definition v0_v1_v2_v3 := [v0; v1; v2; v3].
-Definition adderTree4_v0_v1_v2_v3 := combinational (adderTree4 false v0_v1_v2_v3).
-Example sum_v0_v1_v2_v3 : Bv2N (combinational (adderTree4 false v0_v1_v2_v3)) = 30.
+Definition adderTree4_v0_v1_v2_v3 := combinational (adderTree4 v0_v1_v2_v3).
+Example sum_v0_v1_v2_v3 : Bv2N (combinational (adderTree4 v0_v1_v2_v3)) = 30.
 Proof. reflexivity. Qed.
 
 Local Open Scope nat_scope.
 
 Definition adder_tree_Interface name nrInputs bitSize
   := combinationalInterface name
-     (mkPort "inputs" (Vec (Vec Bit bitSize) nrInputs))
-     (mkPort "sum" (Vec Bit bitSize))
+     [mkPort "inputs" (Vec (Vec Bit bitSize) nrInputs)]
+     [mkPort "sum" (Vec Bit bitSize)]
      [].
 
 (* Create netlist and test-bench for a 4-input adder tree. *)
@@ -100,7 +100,7 @@ Definition adder_tree_Interface name nrInputs bitSize
 Definition adder_tree4_8Interface := adder_tree_Interface "xadder_tree4_8" 4 8.
 
 Definition adder_tree4_8Netlist
-  := makeNetlist adder_tree4_8Interface (adderTree4 Gnd).
+  := makeNetlist adder_tree4_8Interface adderTree4.
 
 Local Open Scope N_scope.
 
@@ -111,7 +111,7 @@ Definition adder_tree4_8_tb_inputs
       [9; 56; 2; 87];   [14; 72; 90; 11]; [64; 12; 92; 13];    [88; 24; 107; 200]]).
 
 Definition adder_tree4_8_tb_expected_outputs
-  := map (fun i => combinational (adderTree4 false i)) adder_tree4_8_tb_inputs.
+  := map (fun i => combinational (adderTree4 i)) adder_tree4_8_tb_inputs.
 
 Definition adder_tree4_8_tb :=
   testBench "xadder_tree4_8_tb" adder_tree4_8Interface
@@ -131,21 +131,21 @@ Proof. reflexivity. Qed.
 Definition adder_tree32_8Interface := adder_tree_Interface "xadder_tree32_8" 32 8.
 
 Definition adder_tree32_8Netlist
-  := makeNetlist adder_tree32_8Interface (adderTree Gnd 4).
+  := makeNetlist adder_tree32_8Interface (adderTree 4).
 
 (* Create netlist and test-bench for a 64-input adder tree. *)
 
 Definition adder_tree64_8Interface := adder_tree_Interface "xadder_tree64_8" 64 8.
 
 Definition adder_tree64_8Netlist
-  := makeNetlist adder_tree64_8Interface (adderTree Gnd 5).
+  := makeNetlist adder_tree64_8Interface (adderTree 5).
 
 Definition adder_tree64_8_tb_inputs
   := map (fun i => Vector.map (N2Bv_sized 8) (Vector.map N.of_nat i))
      [vseq 0 64; vseq 64 64; vseq 128 64].
 
 Definition adder_tree64_8_tb_expected_outputs
-  := map (fun i => combinational (adderTree false 5 i)) adder_tree64_8_tb_inputs.
+  := map (fun i => combinational (adderTree 5 i)) adder_tree64_8_tb_inputs.
 
 Definition adder_tree64_8_tb :=
   testBench "xadder_tree64_8_tb" adder_tree64_8Interface
@@ -158,7 +158,7 @@ Definition adder_tree64_8_tb :=
 Definition adder_tree64_128Interface := adder_tree_Interface "xadder_tree64_128" 64 128.
 
 Definition adder_tree64_128Netlist
-  := makeNetlist adder_tree64_128Interface (adderTree Gnd 5).
+  := makeNetlist adder_tree64_128Interface (adderTree 5).
 
 Definition adder_tree64_128_tb_inputs
   := map (fun i => Vector.map (N2Bv_sized 128) i)
@@ -166,7 +166,7 @@ Definition adder_tree64_128_tb_inputs
      [vseq 0 64; vseq 64 64; vseq 128 64]).
 
 Definition adder_tree64_128_tb_expected_outputs
-  := map (fun i => combinational (adderTree false 5 i)) adder_tree64_128_tb_inputs.
+  := map (fun i => combinational (adderTree 5 i)) adder_tree64_128_tb_inputs.
 
 Definition adder_tree64_128_tb :=
   testBench "xadder_tree64_128_tb" adder_tree64_128Interface
@@ -179,7 +179,7 @@ Definition adder_tree64_128_tb :=
 Definition adder_tree128_256Interface := adder_tree_Interface "xadder_tree128_256" 128 256.
 
 Definition adder_tree128_256Netlist
-  := makeNetlist adder_tree128_256Interface (adderTree Gnd 6).
+  := makeNetlist adder_tree128_256Interface (adderTree 6).
 
 Definition adder_tree128_256_tb_inputs : list (Vector.t (Bvector 256) 128)
   := map (fun i => Vector.map (N2Bv_sized 256) i)
@@ -188,7 +188,7 @@ Definition adder_tree128_256_tb_inputs : list (Vector.t (Bvector 256) 128)
 
 Definition adder_tree128_256_tb_expected_outputs
            : list (Bvector 256)
-  := map (fun i => combinational (adderTree false 6 i)) adder_tree128_256_tb_inputs.
+  := map (fun i => combinational (adderTree 6 i)) adder_tree128_256_tb_inputs.
 
 Definition adder_tree128_256_tb :=
   testBench "xadder_tree128_256_tb" adder_tree128_256Interface
