arrow-examples/Mux2_1.v
@@ -46,15 +46,10 @@ Proof. simply_combinational. Qed.
 
 Require Import Cava.Types.
 Require Import Cava.Netlist.
-
-Definition mux2_1_Interface :=
-   combinationalInterface "mux2_1"
-     (mkPort "s" Kind.Bit, (mkPort "a" Kind.Bit, mkPort "b" Kind.Bit))
-     (mkPort "o" Kind.Bit)
-     [].
+Require Import Cava.Signal.
 
 Definition mux2_1_netlist :=
-  makeNetlist mux2_1_Interface (build_netlist (closure_conversion mux2_1)).
+  build_netlist (closure_conversion mux2_1) "mux2_1" ("s", ("a", "b")) "o".
 
 Definition mux2_1_tb_inputs : list (bool * (bool * bool)) :=
  [(false, (false, true));
@@ -70,5 +65,8 @@ Definition mux2_1_tb_expected_outputs : list bool :=
 Goal is_combinational (closure_conversion mux2_1). Proof. simply_combinational. Qed.
 
 Definition mux2_1_tb :=
-  testBench "mux2_1_tb" mux2_1_Interface
-            mux2_1_tb_inputs mux2_1_tb_expected_outputs.
+  testBench "mux2_1_tb"
+   (combinationalInterface "mux2_1"
+     [mkPort "s" Bit; mkPort "a" Bit; mkPort "b" Bit]
+     [mkPort "o" Bit] [])
+  (map (fun '(a,(b,c)) => (a,b,c)) mux2_1_tb_inputs) mux2_1_tb_expected_outputs.
