cava/Cava/Monad/UnsignedAdders.v
@@ -22,44 +22,49 @@ Require Import Cava.Cava.
 From Cava Require Import Kind.
 Require Import Cava.Monad.CavaMonad.
 
-(******************************************************************************)
-(* An adder with two inputs of the same size and no bit-growth                *)
-(******************************************************************************)
+Section WithCava.
+  Context {signal} `{Cava signal} `{Monad cava}.
 
-Lemma n_le_n_plus_1 : forall n, 0 + n <= 1 + n.
-Proof. auto. Defined.
+  (****************************************************************************)
+  (* An adder with two inputs of the same size and no bit-growth              *)
+  (****************************************************************************)
 
-Lemma max_n_n : forall n, max n n = n.
-Proof.
-  intros.
-  induction n.
-  - reflexivity.
-  - simpl. rewrite IHn. reflexivity.
-Defined.
+  Lemma n_le_n_plus_1 : forall n, 0 + n <= 1 + n.
+  Proof. auto. Defined.
 
-Definition deMax {m bit} `{Cava m bit} {n} (v: Vector.t bit (1 + max n n)) :
-                 Vector.t (smashTy bit Bit) (1+n).
-Proof.
-  rewrite max_n_n in v.
-  unfold smashTy. apply v.
-Defined.
+  Lemma max_n_n : forall n, max n n = n.
+  Proof.
+    intros.
+    induction n.
+    - reflexivity.
+    - simpl. rewrite IHn. reflexivity.
+  Defined.
 
-Definition addN {m bit} `{Cava m bit} {n}
-                (a: Vector.t bit n) (b: Vector.t bit n) : m (Vector.t bit n) :=
-  s <- unsignedAdd a b ;;
-  ret (slice 0 n (deMax s) (n_le_n_plus_1 _)).
+  Definition deMax {n} (v: signal (Vec Bit (1 + max n n))) :
+                       signal (Vec Bit (1+n)).
+  Proof.
+    rewrite max_n_n in v.
+    apply v.
+  Defined.
 
-(******************************************************************************)
-(* A three input adder.                                                       *)
-(******************************************************************************)
+  Definition addN {n: nat}
+                  (a b: signal (Vec Bit n))
+                  : cava (signal (Vec Bit n)) :=
+    s <- unsignedAdd a b ;;
+    ret (slice 0 n (deMax s) (n_le_n_plus_1 _)).
 
-Definition adder_3input {m bit} `{Cava m bit}
-                        {aSize bSize cSize}
-                        (a : Vector.t bit aSize)
-                        (b : Vector.t bit bSize)
-                        (c : Vector.t bit cSize) :
-                        m (Vector.t bit (1 + max (1 + max aSize bSize) cSize))
-                        :=
-  a_plus_b <- unsignedAdd a b ;;
-  sum <- unsignedAdd a_plus_b c ;;
-  ret sum.
+  (****************************************************************************)
+  (* A three input adder.                                                     *)
+  (****************************************************************************)
+
+  Definition adder_3input {aSize bSize cSize}
+                          (a : signal (Vec Bit aSize))
+                          (b : signal (Vec Bit bSize))
+                          (c : signal (Vec Bit cSize)) :
+                          cava (signal (Vec Bit (1 + max (1 + max aSize bSize) cSize)))
+                          :=
+    a_plus_b <- unsignedAdd a b ;;
+    sum <- unsignedAdd a_plus_b c ;;
+    ret sum.
+
+ End WithCava.
